checkpoint; non-decidable partiality for PCMs

ulib/experimental/Steel.PCM.Memory.fst
@@ -25,7 +25,6 @@ type cell : Type u#(a + 1) =
   | Ref : a:Type u#a ->
           p:pcm a ->
           v:a ->
-          squash (defined p v) ->
           cell
 
 let addr = nat
@@ -47,24 +46,18 @@ let update_addr (m:heap) (a:addr) (c:cell)
   : heap
   = F.on _ (fun a' -> if a = a' then Some c else m a')
 
-let combinable_sym (#a:Type) (pcm:pcm a) (x y: a)
-  : Lemma (combinable pcm x y ==>
-           combinable pcm y x)
-  = pcm.comm x y
-
 let disjoint_cells (c0 c1:cell u#h) : prop =
-    let Ref t0 p0 v0 _ = c0 in
-    let Ref t1 p1 v1 _ = c1 in
+    let Ref t0 p0 v0 = c0 in
+    let Ref t1 p1 v1 = c1 in
     t0 == t1 /\
     p0 == p1 /\
-    combinable p0 v0 v1
+    composable p0 v0 v1
 
 let disjoint_cells_sym (c0 c1:cell u#h)
   : Lemma (requires disjoint_cells c0 c1)
           (ensures disjoint_cells c1 c0)
-  = let Ref t0 p0 v0 _ = c0 in
-    let Ref t1 p1 v1 _ = c1 in
-    p0.comm v0 v1
+  = let Ref t0 p0 v0 = c0 in
+    let Ref t1 p1 v1 = c1 in ()
 
 let disjoint_addr (m0 m1:heap u#h) (a:addr)
   : prop
@@ -96,9 +89,9 @@ let disjoint_sym (m0 m1:heap u#h)
     ()
 
 let join_cells (c0:cell u#h) (c1:cell u#h{disjoint_cells c0 c1}) =
-  let Ref a0 p0 v0 _ = c0 in
-  let Ref a1 p1 v1 _ = c1 in
-  Ref a0 p0 (p0.op v0 v1) ()
+  let Ref a0 p0 v0 = c0 in
+  let Ref a1 p1 v1 = c1 in
+  Ref a0 p0 (op p0 v0 v1)
 
 let join (m0:heap) (m1:heap{disjoint m0 m1})
   : heap
@@ -117,15 +110,9 @@ let disjoint_join_cells_assoc (c0 c1 c2:cell u#h)
     (ensures  disjoint_cells c0 c1 /\
               disjoint_cells (join_cells c0 c1) c2 /\
               join_cells (join_cells c0 c1) c2 == join_cells c0 (join_cells c1 c2))
-  = let Ref a0 p0 v0 _ = c0 in
-    let Ref a1 p1 v1 _ = c1 in
-    let Ref a2 p2 v2 _ = c2 in
-    assert (p0 == p1 /\ p1 == p2);
-    assert (p0.op v1 v2 =!= p0.undef);
-    assert (p0.op v0 (p0.op v1 v2) =!= p0.undef);
-    p0.undef_inv v1 v2;
-    p0.undef_inv v0 (p0.op v1 v2);
-    p0.undef_inv (p0.op v0 v1) v2;
+  = let Ref a0 p0 v0 = c0 in
+    let Ref a1 p1 v1 = c1 in
+    let Ref a2 p2 v2 = c2 in
     p0.assoc v0 v1 v2
 
 let disjoint_join' (m0 m1 m2:heap u#h)
@@ -167,8 +154,8 @@ let mem_equiv_eq (m0 m1:heap)
 let join_cells_commutative (c0:cell u#h) (c1:cell u#h{disjoint_cells c0 c1})
   : Lemma (disjoint_cells_sym c0 c1; join_cells c0 c1 == join_cells c1 c0)
           [SMTPat (join_cells c0 c1)]
-  = let Ref a0 p0 v0 _ = c0 in
-    let Ref a1 p1 v1 _ = c1 in
+  = let Ref a0 p0 v0 = c0 in
+    let Ref a1 p1 v1 = c1 in
     p0.comm v0 v1
 
 let join_commutative' (m0 m1:heap)
@@ -268,7 +255,7 @@ type slprop : Type u#(a + 1) =
   | All    : #a:Type u#a -> (a -> slprop u#a) -> slprop
 
 let interp_cell (p:slprop u#a) (c:cell u#a) =
-  let Ref a' pcm' v' _ = c in
+  let Ref a' pcm' v' = c in
   match p with
   | Pts_to #a #pcm r v ->
     a == a' /\
@@ -338,13 +325,25 @@ let intro_pts_to (#a:_) (#pcm:pcm a) (x:ref a pcm) (v:a) (m:heap)
   : Lemma
     (requires
        m `contains_addr` x /\
-       (let Ref a' pcm' v' _ = select_addr m x in
+       (let Ref a' pcm' v' = select_addr m x in
         a == a' /\
         pcm == pcm' /\
         compatible pcm v v'))
      (ensures
        interp (pts_to x v) m)
   = ()
+
+
+let lem_assoc_r #a (p:pcm a) (x y z:a) :
+  Lemma
+    (requires
+       composable p x y /\
+       composable p (op p x y) z)
+    (ensures
+       composable p y z /\
+       composable p x (op p y z) /\
+       op p x (op p y z) == op p (op p x y) z)
+  = admit()
 
 let pts_to_compatible (#a:Type u#a)
                       (#pcm:_)
@@ -355,10 +354,10 @@ let pts_to_compatible (#a:Type u#a)
     (requires
       interp (pts_to x v0 `star` pts_to x v1) m)
     (ensures
-      combinable pcm v0 v1 /\
-      interp (pts_to x (pcm.op v0 v1)) m)
+      composable pcm v0 v1 /\
+      interp (pts_to x (op pcm v0 v1)) m)
   = let c = select_addr m x in
-    let Ref _ _ v _ = select_addr m x in
+    let Ref _ _ v = select_addr m x in
     let aux (c0 c1: cell u#a)
       : Lemma
         (requires
@@ -367,37 +366,41 @@ let pts_to_compatible (#a:Type u#a)
            interp_cell (pts_to x v1) c1 /\
            c == join_cells c0 c1 )
         (ensures
-           combinable pcm v0 v1 /\
-           interp (pts_to x (pcm.op v0 v1)) m)
+           composable pcm v0 v1 /\
+           interp (pts_to x (op pcm v0 v1)) m)
         [SMTPat (c0 `disjoint_cells` c1)]
-      = let Ref _ _ v0' _ = c0 in
-        let Ref _ _ v1' _ = c1 in
-        assert (exists frame. pcm.op frame v0 == v0');
-        assert (exists frame. pcm.op frame v1 == v1');
-        assert (pcm.op v0' v1' == v);
-        assert (v =!= pcm.undef);
+      = let Ref _ _ v0' = c0 in
+        let Ref _ _ v1' = c1 in
+        assert (exists frame. composable pcm v0 frame /\ op pcm frame v0 == v0');
+        assert (exists frame. composable pcm v1 frame /\ op pcm frame v1 == v1');
+        assert (composable pcm v0' v1');
+        assert (op pcm v0' v1' == v);
         let aux (frame0 frame1:a)
           : Lemma
             (requires
-              pcm.op frame0 v0 == v0' /\
-              pcm.op frame1 v1 == v1' /\
-              pcm.op v0' v1' == v)
+              composable pcm v0 frame0 /\
+              op pcm frame0 v0 == v0' /\
+              composable pcm v1 frame1 /\
+              op pcm frame1 v1 == v1')
             (ensures (
-              let frame = pcm.op frame0 frame1 in
-              pcm.op frame (pcm.op v0 v1) == v /\
-              pcm.op v0 v1 =!= pcm.undef))
-            [SMTPat(pcm.op frame0 v0);
-             SMTPat(pcm.op frame1 v1)]
-          = assert (pcm.op (pcm.op frame0 v0) (pcm.op frame1 v1) == v);
-            pcm.assoc frame0 v0 (pcm.op frame1 v1);
-            assert (pcm.op frame0 (pcm.op v0 (pcm.op frame1 v1)) == v);
-            pcm.comm frame1 v1;
-            assert (pcm.op frame0 (pcm.op v0 (pcm.op v1 frame1)) == v);
-            pcm.assoc v0 v1 frame1;
-            assert (pcm.op frame0 (pcm.op (pcm.op v0 v1) frame1) == v);
-            pcm.comm (pcm.op v0 v1) frame1;
-            pcm.assoc frame0 frame1 (pcm.op v0 v1);
-            pcm.undef_inv (pcm.op frame0 frame1) (pcm.op v0 v1)
+              composable pcm frame0 frame1 /\
+              composable pcm v0 v1 /\
+              (let frame = op pcm frame0 frame1 in
+               composable pcm frame (op pcm v0 v1) /\
+               op pcm frame (op pcm v0 v1) == v)))
+            [SMTPat(op pcm frame0 v0);
+             SMTPat(op pcm frame1 v1)]
+          =  assert (op pcm (op pcm frame0 v0) (op pcm frame1 v1) == v);
+             pcm.assoc (op pcm frame0 v0) frame1 v1;
+             assert (op pcm (op pcm (op pcm frame0 v0) frame1) v1 == v);
+             pcm.comm  (op pcm frame0 v0) frame1;
+             assert (op pcm (op pcm frame1 (op pcm frame0 v0)) v1 == v);
+             lem_assoc_r pcm frame1 (op pcm frame0 v0) v1;
+             assert (op pcm frame1 (op pcm (op pcm frame0 v0) v1) == v);
+             lem_assoc_r pcm frame0 v0 v1;
+             assert (op pcm frame1 (op pcm frame0 (op pcm v0 v1)) == v);
+             pcm.assoc frame1 frame0 (op pcm v0 v1);
+             pcm.comm frame1 frame0
         in
         ()
     in
@@ -478,14 +481,13 @@ let star_congruence (p1 p2 p3 p4:slprop) = ()
 ////////////////////////////////////////////////////////////////////////////////
 let sel #a #pcm (r:ref a pcm) (m:hheap (ptr r))
   : a
-  = let Ref _ _ v _ = select_addr m r in
+  = let Ref _ _ v = select_addr m r in
     v
 
 let sel_lemma (#a:_) (#pcm:_) (r:ref a pcm) (m:hheap (ptr r))
   : Lemma (interp (pts_to r (sel r m)) m)
-  = let Ref _ _ v _ = select_addr m r in
+  = let Ref _ _ v = select_addr m r in
     assert (sel r m == v);
-    assert (defined pcm v);
     compatible_refl pcm v
 
 let sel_action (#a:_) (#pcm:_) (r:ref a pcm) (v0:erased a)
@@ -499,19 +501,18 @@ let sel_action (#a:_) (#pcm:_) (r:ref a pcm) (v0:erased a)
     f
 
 
-let update_defined #a pcm (v0:a{defined pcm v0}) (v1:a{frame_preserving pcm v0 v1})
-  : Lemma (defined pcm v1)
-  = pcm.is_unit v0; pcm.is_unit v1;
-    assert (defined pcm (pcm.op v0 pcm.one));
-    pcm.comm v0 pcm.one;
-    pcm.comm v1 pcm.one;
-    assert (defined pcm v1)
+// let update_defined #a pcm (v0:a) (v1:a{frame_preserving pcm v0 v1})
+//   : Lemma (defined pcm v1)
+//   = pcm.is_unit v0; pcm.is_unit v1;
+//     assert (defined pcm (pcm.op v0 pcm.one));
+//     pcm.comm v0 pcm.one;
+//     pcm.comm v1 pcm.one;
+//     assert (defined pcm v1)
 
 let upd' (#a:_) (#pcm:_) (r:ref a pcm) (v0:FStar.Ghost.erased a) (v1:a {frame_preserving pcm v0 v1})
   : pre_action (pts_to r v0) unit (fun _ -> pts_to r v1)
   = fun h ->
-    update_defined pcm v0 v1;
-    let cell = Ref a pcm v1 () in
+    let cell = Ref a pcm v1  in
     let h' = update_addr h r cell in
     assert (h' `contains_addr` r);
     compatible_refl pcm v1;
@@ -520,60 +521,49 @@ let upd' (#a:_) (#pcm:_) (r:ref a pcm) (v0:FStar.Ghost.erased a) (v1:a {frame_pr
     (| (), h' |)
 
 
-let definedness #a #pcm (v0:a{defined pcm v0}) (v0_val:a{defined pcm v0_val}) (v1:a{defined pcm v1}) (vf:a{defined pcm vf})
+let definedness #a #pcm (v0:a) (v0_val:a) (v1:a) (vf:a)
   : Lemma (requires
              compatible pcm v0 v0_val /\
-             combinable pcm v0_val vf /\
+             composable pcm v0_val vf /\
              frame_preserving pcm v0 v1)
           (ensures
-             combinable pcm vf v1 /\
-             combinable pcm v1 vf)
-  = assert (exists vf'. pcm.op vf' v0 == v0_val);
-    let aux (vf':a {pcm.op vf' v0 == v0_val})
-      : Lemma (combinable pcm vf v1 /\
-               combinable pcm v1 vf)
-              [SMTPat(pcm.op vf' v0)]
-        = pcm.undef_inv vf' v0;
-          assert (defined pcm vf');
-          assert (combinable pcm (pcm.op vf' v0) vf);
-          pcm.comm (pcm.op vf' v0) vf;
-          pcm.assoc vf vf' v0;
-          pcm.comm (pcm.op vf vf') v0;
-          assert (combinable pcm v0 (pcm.op vf vf'));
-          pcm.comm v0 (pcm.op vf vf');
-          assert (combinable pcm (pcm.op vf vf') v1);
-          pcm.comm (pcm.op vf vf') v1;
+             composable pcm vf v1 /\
+             composable pcm v1 vf)
+  = assert (exists vf'. composable pcm vf' v0 /\ op pcm vf' v0 == v0_val);
+    let aux (vf':a {composable pcm vf' v0 /\ op pcm vf' v0 == v0_val})
+      : Lemma (composable pcm vf v1 /\
+               composable pcm v1 vf)
+              [SMTPat(op pcm vf' v0)]
+        = assert (composable pcm (op pcm vf' v0) vf);
+          pcm.comm vf' v0;
+          assert (composable pcm (op pcm v0 vf') vf);
+          lem_assoc_r pcm v0 vf' vf;
+          assert (composable pcm v0 (op pcm vf' vf));
+          pcm.comm vf vf';
+          assert (composable pcm v0 (op pcm vf vf'));
+          assert (composable pcm (op pcm vf vf') v1);
+          pcm.comm (op pcm vf vf') v1;
           pcm.assoc v1 vf vf';
-          assert (combinable pcm (pcm.op v1 vf) vf');
-          pcm.undef_inv v1 vf;
-          pcm.undef_inv (pcm.op v1 vf) vf';
-          assert (combinable pcm v1 vf);
-          pcm.comm v1 vf;
-          assert (combinable pcm vf v1)
+          assert (composable pcm (op pcm v1 vf) vf')
     in
     ()
 
-let combinable_compatible #a pcm (x y z:a)
+let composable_compatible #a pcm (x y z:a)
   : Lemma (requires compatible pcm x y /\
-                    combinable pcm y z)
-          (ensures combinable pcm x z /\
-                   combinable pcm z x)
-  = let aux (f:a{pcm.op f x == y})
-      : Lemma (combinable pcm x z /\
-               combinable pcm z x)
-              [SMTPat (pcm.op f x)]
-      = assert (combinable pcm (pcm.op f x) z);
-        pcm.assoc f x z;
-        assert (combinable pcm f (pcm.op x z));
-        pcm.undef_inv f (pcm.op x z);
+                    composable pcm y z)
+          (ensures composable pcm x z /\
+                   composable pcm z x)
+  = let aux (f:a{composable pcm f x /\ op pcm f x == y})
+      : Lemma (composable pcm x z /\
+               composable pcm z x)
+              [SMTPat (op pcm f x)]
+      = assert (composable pcm (op pcm f x) z);
+        lem_assoc_r pcm f x z;
+        assert (composable pcm f (op pcm x z));
         pcm.comm x z
     in
-    let s : squash (exists f. pcm.op f x == y) = () in
+    let s : squash (exists f. composable pcm f x /\ op pcm f x == y) = () in
     ()
-
-let pts_to_defined #a #pcm (r:ref a pcm) (v:a) (m:hheap (pts_to r v))
-  : Lemma (defined pcm v)
-  = ()
 
 #push-options "--z3rlimit_factor 2"
 let upd_lemma' (#a:_) #pcm (r:ref a pcm)
@@ -585,8 +575,7 @@ let upd_lemma' (#a:_) #pcm (r:ref a pcm)
     (ensures (
       (let (| x, h1 |) = upd' r v0 v1 h in
        interp (pts_to r v1 `star` frame) h1)))
-  = assert (defined pcm v0); update_defined pcm v0 v1;
-    let aux (h0 hf:heap)
+  = let aux (h0 hf:heap)
      : Lemma
        (requires
          disjoint h0 hf /\
@@ -595,14 +584,14 @@ let upd_lemma' (#a:_) #pcm (r:ref a pcm)
          interp frame hf)
        (ensures (
          let (| _, h' |) = upd' r v0 v1 h in
-         let h0' = update_addr h0 r (Ref a pcm v1 ()) in
+         let h0' = update_addr h0 r (Ref a pcm v1) in
          disjoint h0' hf /\
          interp (pts_to r v1) h0' /\
          interp frame hf /\
          h' == join h0' hf))
        [SMTPat (disjoint h0 hf)]
      = let (| _, h'|) = upd' r v0 v1 h in
-       let cell1 = (Ref a pcm v1 ()) in
+       let cell1 = (Ref a pcm v1) in
        let h0' = update_addr h0 r cell1 in
        assert (interp (pts_to r v1) h0');
        assert (interp frame hf);
@@ -611,9 +600,9 @@ let upd_lemma' (#a:_) #pcm (r:ref a pcm)
                  [SMTPat (disjoint_addr h0' hf a)]
          = if a <> r then ()
            else match h0 a, h0' a, hf a with
-                | Some (Ref a0 p0 v0_val _),
-                  Some (Ref a0' p0' v0' _),
-                  Some (Ref af pf vf _) ->
+                | Some (Ref a0 p0 v0_val),
+                  Some (Ref a0' p0' v0'),
+                  Some (Ref af pf vf) ->
                   assert (a0' == af);
                   assert (p0' == pf);
                   assert (v0' == v1);
@@ -628,13 +617,12 @@ let upd_lemma' (#a:_) #pcm (r:ref a pcm)
                   assert (interp (pts_to r v0_val) h0);
                   assert (interp (pts_to r v0_val `star` pts_to r vf) h);
                   pts_to_compatible r v0_val vf h;
-                  assert (combinable pcm v0_val vf);
+                  assert (composable pcm v0_val vf);
 
-                  assert (interp (pts_to r (pcm.op v0_val vf)) h);
+                  assert (interp (pts_to r (op pcm v0_val vf)) h);
                   pcm.comm v0_val vf;
-                  assert (defined pcm (pcm.op vf v0_val));
                   definedness #_ #pcm v0 v0_val v1 vf;
-                  assert (combinable pcm v1 vf)
+                  assert (composable pcm v1 vf)
                 | _ -> ()
        in
        assert (disjoint h0' hf);
@@ -648,21 +636,21 @@ let upd_lemma' (#a:_) #pcm (r:ref a pcm)
              assert (h0' a == Some cell1);
              match h0 a, hf a with
              | _, None -> ()
-             | Some (Ref a0 p0 v0_val _),
-               Some (Ref af pf vf _) ->
+             | Some (Ref a0 p0 v0_val),
+               Some (Ref af pf vf) ->
                let c0 = Some?.v (h0 a) in
                let cf = Some?.v (hf a) in
                assert (a0 == af);
                assert (p0 == pf);
                assert (compatible pcm v0 v0_val);
                assert (disjoint_cells c0 cf);
-               assert (combinable pcm v0_val vf);
-               combinable_compatible pcm v0 v0_val vf;
-               assert (combinable pcm v0 vf);
+               assert (composable pcm v0_val vf);
+               composable_compatible pcm v0 v0_val vf;
+               assert (composable pcm v0 vf);
                assert (disjoint_cells cell1 cf);
-               assert (combinable pcm v1 vf);
-               assert (combinable pcm vf v0);
-               assert (pcm.op vf v1 == v1);
+               assert (composable pcm v1 vf);
+               assert (composable pcm vf v0);
+               assert (op pcm vf v1 == v1);
                pcm.comm vf v1
            end
        in
