ulib/experimental/Steel.PCM.fst
@@ -1,51 +1,59 @@
 module Steel.PCM
 
-let commutative #a (op:a -> a -> a) = forall x y. op x y == op y x
-let associative #a (op:a -> a -> a) = forall x y z. (op x (op y z) == op (op x y) z)
-let is_unit #a (op:a -> a -> a) (u:a) = forall x. op x u == x
-let is_undef #a (op:a -> a -> a) (z:a) = forall x. op x z == z
-let undef_inv #a (op:a -> a -> a) (z:a) = forall x y. op x y =!= z ==> x =!= z /\ y =!= z
+// let commutative #a (op:a -> a -> a) = forall x y. op x y == op y x
+// let associative #a (op:a -> a -> a) = forall x y z. (op x (op y z) == op (op x y) z)
 
-let lem_commutative #a (op:a -> a -> a) = (x:a) -> (y:a) -> Lemma (op x y == op y x)
-let lem_associative #a (op: a -> a -> a) = x:a -> y:a -> z:a -> Lemma (op x (op y z) == op (op x y) z)
-let lem_is_unit #a (op:a -> a -> a) (u:a) = x:a -> Lemma (op x u == x)
-let lem_is_undef #a (op:a -> a -> a) (z:a) = x:a -> Lemma (op x z == z)
-let lem_undef_inv #a (op:a -> a -> a) (z:a) = x:a -> y:a -> Lemma (op x y =!= z ==> x =!= z /\ y =!= z)
+// let is_unit #a (op:a -> a -> a) (u:a) = forall x. op x u == x
+// let is_undef #a (op:a -> a -> a) (z:a) = forall x. op x z == z
+// let undef_inv #a (op:a -> a -> a) (z:a) = forall x y. op x y =!= z ==> x =!= z /\ y =!= z
 
+let symrel a = c:(a -> a -> prop) { (forall x y. c x y <==> c y x) }
+
+noeq
+type pcm' (a:Type) = {
+  composable: symrel a;
+  op: x:a -> y:a{composable x y} -> a;
+  one:a
+}
+
+let lem_commutative #a (p:pcm' a) =
+  x:a ->
+  y:a{p.composable x y} ->
+  Lemma (p.op x y == p.op y x)
+
+let lem_associative #a (p:pcm' a) =
+  x:a ->
+  y:a ->
+  z:a{p.composable y z /\ p.composable x (p.op y z)} ->
+  Lemma (p.composable x y /\
+         p.composable (p.op x y) z /\
+         p.op x (p.op y z) == p.op (p.op x y) z)
+
+let lem_is_unit #a (p:pcm' a) =
+  x:a ->
+  Lemma (p.composable x p.one /\
+         p.op x p.one == x)
 
 noeq
 type pcm (a:Type) = {
-  op: a -> a -> a;
-  one:a;
-  undef:a;
-  laws: unit -> squash (commutative op /\
-                       associative op /\
-                       is_unit op one /\
-                       is_undef op undef /\
-                       undef_inv op undef);
-  comm:lem_commutative op;
-  assoc:lem_associative op;
-  is_unit:lem_is_unit op one;
-  is_undef:lem_is_undef op undef;
-  undef_inv:lem_undef_inv op undef;
+  p:pcm' a;
+  comm:lem_commutative p;
+  assoc: lem_associative p;
+  is_unit: lem_is_unit p
 }
 
-let defined #a (pcm:pcm a) (x:a) = x =!= pcm.undef
-
-let combinable (#a:Type) (pcm:pcm a) (x y: a) =
-  pcm.op x y =!= pcm.undef
-
+let composable #a (p:pcm a) (x y:a) = p.p.composable x y
+let op #a (p:pcm a) (x:a) (y:a{composable p x y}) = p.p.op x y
 let compatible #a (pcm:pcm a) (x y:a) =
-  defined pcm x /\
-  defined pcm y /\
-  (exists (frame:a). pcm.op frame x == y)
+  (exists (frame:a). composable pcm x frame /\
+                op pcm frame x == y)
 
-let compatible_refl #a (pcm:pcm a) (x:a{defined pcm x})
+let compatible_refl #a (pcm:pcm a) (x:a)
   : Lemma (compatible pcm x x)
   = pcm.is_unit x;
-    pcm.comm x pcm.one;
-    assert (pcm.op pcm.one x == x)
+    pcm.comm x pcm.p.one;
+    assert (op pcm pcm.p.one x == x)
 
 let frame_preserving #a (pcm:pcm a) (x y: a) =
-    (forall frame. combinable pcm frame x ==> combinable pcm frame y) /\
-    (forall frame.{:pattern (combinable pcm frame x)} combinable pcm frame x ==> pcm.op frame y == y)
+    (forall frame. composable pcm frame x ==> composable pcm frame y) /\
+    (forall frame.{:pattern (composable pcm frame x)} composable pcm frame x ==> op pcm frame y == y)
